Clean up locations.v.

theories/semantics/locations.v
@@ -1,40 +1,46 @@
 From stdpp Require Import countable numbers gmap.
 
-(* TODO:
-   - add the required lemmas so that the types declared below can remain opaque
-     to the rest of the development. *)
+Local Open Scope Z_scope.
 
-(* The following section comes from the file
-   [iris_heap_lang/locations.v] available in the [iris] repository. *)
+(* A location is an integer. *)
 
-Section Locations.
+Definition loc := Z.
 
-  Record loc := Loc { loc_car : Z }.
+(* If needed, one could declare instances of the type classes [EqDecision],
+   [Inhabited], [Countable], [Infinite] for the type [loc]. *)
 
-  Add Printing Constructor loc.
+(* [max_loc ls] computes an upper bound of the finite set of locations [ls].
+   It is in the fact the least upper bound of the set [ls], except when [ls]
+   is empty. *)
 
-  Global Instance loc_eq_decision : EqDecision loc.
-  Proof. solve_decision. Defined.
+Definition max_loc (ls : gset loc) : loc :=
+  set_fold Z.max 0 ls.
 
-  Global Instance loc_inhabited : Inhabited loc := populate {|loc_car := 0 |}.
+Lemma le_max_loc :
+  ∀ ls l, l ∈ ls → l ≤ max_loc ls.
+Proof.
+  apply (set_fold_ind_L (λ r ls, ∀ l, l ∈ ls → l ≤ r)).
+  { set_solver. }
+  { intros x X r _ IH l.
+    rewrite elem_of_union, Z.max_le_iff.
+    set_solver by eauto with lia. }
+Qed.
 
-  Global Instance loc_countable : Countable loc.
-  Proof. by apply (inj_countable' loc_car Loc); intros []. Defined.
+(* [fresh_loc ls] is a location that is guaranteed not to be a member of the
+   finite set of locations [ls]. *)
 
-  Global Program Instance loc_infinite : Infinite loc :=
-    inj_infinite (λ p, {| loc_car := p |}) (λ l, Some (loc_car l)) _.
-  Next Obligation. done. Qed.
+Definition fresh_loc (ls : gset loc) : loc :=
+  max_loc ls + 1.
 
-  Definition fresh_locs (ls : gset loc) : loc :=
-    {| loc_car := set_fold (λ k r, (1 + loc_car k) `max` r)%Z 1%Z ls |}.
+Lemma fresh_loc_fresh ls :
+  fresh_loc ls ∉ ls.
+Proof.
+  unfold fresh_loc.
+  intro H.
+  specialize (le_max_loc _ _ H); clear H; intro H.
+  lia.
+Qed.
 
-  Lemma fresh_locs_fresh ls :
-    fresh_locs ls ∉ ls.
-  Proof.
-    cut (∀ l, l ∈ ls → loc_car l < loc_car (fresh_locs ls))%Z.
-    { intros help Hf%help. lia. }
-    apply (set_fold_ind_L (λ r ls, ∀ l, l ∈ ls → (loc_car l < r)%Z));
-    set_solver by eauto with lia.
-  Qed.
+(* The type of locations can now be made opaque. *)
 
-End Locations.
+Global Opaque loc.
